Further work on constprop

Leroy/Constprop.lean
@@ -1,6 +1,8 @@
 import «Leroy».Sequences
 import «Leroy».Imp
 import Init.Data.List.Basic
+import Std.Data.HashMap
+import Std.Data.HashMap.Lemmas
 
 set_option grind.debug true
 set_option grind.warning false
@@ -137,3 +139,401 @@ theorem cexec_mk_WHILE_loop: forall b c s1 s2 s3,
   cexec s1 (mk_WHILE b c) s3 := by
     intro b c s1 s2 s3 h1 h2 h3
     fun_cases (mk_WHILE b c) <;> grind
+
+def Store := Std.HashMap ident Int
+@[grind] def matches' (s: store) (S: Store): Prop :=
+  forall x n, S.get? x = .some n -> s x = n
+
+@[grind] def Le (S1 S2: Store) : Prop :=
+  forall x n, S2.get? x = .some n -> S1.get? x = .some n
+
+@[grind] def Top : Store := Std.HashMap.emptyWithCapacity
+
+@[grind] def Join (S1 S2: Store) : Store :=
+  S1.filter (fun key _ => S2.get? key == S1.get? key)
+
+-- In leroy's course this is decidable
+def Equal (S1 S2: Store) := Std.HashMap.Equiv S1 S2
+
+def Equal' (S1 S2 : Store) : Bool := S1.toArray.all (S2.toArray.contains) && S2.toArray.all (S1.toArray.contains)
+
+
+-- (** We show the soundness of these lattice operations with respect to
+--   the [matches] and the [Le] relations. *)
+
+theorem matches_Le: forall s S1 S2, Le S1 S2 -> matches' s S1 -> matches' s S2 := by
+  intro s S1 S2 h1 h2
+  grind
+
+theorem Le_Top: forall S, Le S Top := by
+  intro S
+  grind [Std.HashMap]
+
+@[grind] theorem Join_characterization:
+forall S1 S2 x n,
+  (Join S1 S2).get? x = .some n ↔
+  S1.get? x = .some n ∧ S2.get? x = .some n := by
+  intro S1 S2 x n
+  constructor
+  case mpr =>
+    grind
+  case mp =>
+    sorry
+
+theorem Le_Join_l: forall S1 S2, Le S1 (Join S1 S2) := by intros; grind
+
+theorem  Le_Join_r: forall S1 S2, Le S2 (Join S1 S2) := by intros; grind
+
+theorem Equal_Le: forall S1 S2, Equal S1 S2 -> Le S1 S2 := by
+  intro S1 S2 eq
+  unfold Equal at eq
+  unfold Le
+  intro x n
+  have := @Std.HashMap.Equiv.getElem?_eq _ _ _ _ S1 S2 _ _ x eq
+  grind
+
+@[grind] def lift1 {A B: Type} (f: A -> B) (o: Option A) : Option B :=
+  match o with
+  | .some x => .some (f x)
+  | .none => .none
+
+@[grind] def lift2 {A B C: Type} (f: A -> B -> C) (o1: Option A) (o2: Option B) : Option C :=
+  match o1, o2 with
+  | .some x1, .some x2 => .some (f x1 x2) | _, _ => .none
+
+@[grind] def Aeval (S: Store) (a: aexp) : Option Int :=
+  match a with
+  | .CONST n => .some n
+  | .VAR x => S.get? x
+  | .PLUS a1 a2 => lift2 (Int.add) (Aeval S a1) (Aeval S a2)
+  | .MINUS a1 a2 => lift2 (Int.sub) (Aeval S a1) (Aeval S a2)
+
+@[grind] def Beval (S: Store) (b: bexp) : Option Bool :=
+  match b with
+  | .TRUE => .some true
+  | .FALSE => .some false
+  | .EQUAL a1 a2 => lift2 (fun m n => m == n) (Aeval S a1) (Aeval S a2)
+  | .LESSEQUAL a1 a2 => lift2 (fun m n => m <= n) (Aeval S a1) (Aeval S a2)
+  | .NOT b1 => lift1 (fun m => !m) (Beval S b1)
+  | .AND b1 b2 => lift2 (fun m n => m && n) (Beval S b1) (Beval S b2)
+
+@[grind] theorem Aeval_sound:
+  forall s S, matches' s S ->
+  forall a n, Aeval S a = .some n -> aeval s a = n := by
+    intro s S h1 a n h2
+    induction a generalizing n
+    any_goals grind
+    case PLUS a1 a2 a1_ih a2_ih =>
+      simp [Aeval] at h2
+      unfold lift2 at h2
+      split at h2 <;> grind
+    case MINUS a1 s2 a1_ih a2_ih =>
+      simp [Aeval] at h2
+      unfold lift2 at h2
+      split at h2 <;> grind
+
+theorem Beval_sound:
+  forall s S, matches' s S ->
+  forall b n, Beval S b = .some n -> beval s b = n := by
+    intro s S h1 b n h2
+    induction b generalizing n
+    any_goals grind
+    case EQUAL a1 a2 =>
+      unfold Beval at h2
+      unfold lift2 at h2
+      split at h2
+      any_goals grind
+    case LESSEQUAL a1 a2 =>
+      unfold Beval at h2
+      unfold lift2 at h2
+      split at h2 <;> grind
+    case NOT a1 a1_ih =>
+      unfold Beval at h2
+      unfold lift1 at h2
+      split at h2 <;> grind
+    case AND a1 a2 =>
+      unfold Beval at h2
+      unfold lift2 at h2
+      split at h2 <;> grind
+
+
+@[grind] def Update (x: ident) (N: Option Int) (S: Store) : Store :=
+  match N with
+  | .none => S.erase x
+  | .some n => S.insert x n
+
+@[grind] theorem update_characterisation : forall S x N y,
+  (Update x N S).get? y = if x == y then N else S.get? y := by
+    intro S x N y
+    simp
+    split
+    case isTrue eq =>
+      simp at eq
+      rw [eq]
+      unfold Update
+      grind
+    case isFalse neq =>
+      simp at neq
+      unfold Update
+      grind
+
+theorem matches_update: forall s S x n N,
+  matches' s S ->
+  (forall i, N = .some i -> n = i) ->
+  matches' (update x n s) (Update x N S) := by
+    intro s S x n N m h
+    grind
+
+def fixpoint_rec (F: Store -> Store) (fuel: Nat) (S: Store) : Store :=
+  match fuel with
+  | 0 => Top
+  | fuel + 1 =>
+      let S' := F S
+      if Equal' S' S then S else fixpoint_rec F fuel S'
+
+
+-- (** Let's say that we will do at most 20 iterations. *)
+
+-- Definition num_iter := 20%nat.
+
+-- Definition fixpoint (F: Store -> Store) (init_S: Store) : Store :=
+--   fixpoint_rec F num_iter init_S.
+
+-- (** The result [S] of [fixpoint F] is sound, in that it satisfies
+--     [F S <= S] in the lattice ordering. *)
+
+-- Lemma fixpoint_sound: forall F init_S,
+--   let S := fixpoint F init_S in Le (F S) S.
+-- Proof.
+--   intros F.
+--   assert (A: forall fuel S,
+--              fixpoint_rec F fuel S = Top
+--              \/ Equal (F (fixpoint_rec F fuel S)) (fixpoint_rec F fuel S) = true).
+--   { induction fuel as [ | fuel]; cbn; intros.
+--   - auto.
+--   - destruct (Equal (F S) S) eqn:E.
+--     + auto.
+--     + apply IHfuel.
+--   }
+--   intros.
+--   assert (E: S = Top \/ Equal (F S) S = true) by apply A.
+--   destruct E as [E | E].
+--   - rewrite E.  apply Le_Top.
+--   - apply Equal_Le; auto.
+-- Qed.
+
+-- (** Now we can analyze commands by executing them "in the abstract".
+--   Given an abstract store [S] that represents what we statically know
+--   about the values of the variables before executing command [c],
+--   [cexec'] returns an abstract store that describes the values of
+--   the variables after executing [c]. *)
+
+-- Fixpoint Cexec (S: Store) (c: com) : Store :=
+--   match c with
+--   | SKIP => S
+--   | ASSIGN x a => Update x (Aeval S a) S
+--   | SEQ c1 c2 => Cexec (Cexec S c1) c2
+--   | IFTHENELSE b c1 c2 =>
+--       match Beval S b with
+--       | Some true => Cexec S c1
+--       | Some false => Cexec S c2
+--       | None => Join (Cexec S c1) (Cexec S c2)
+--       end
+--   | WHILE b c1 =>
+--       fixpoint (fun x => Join S (Cexec x c1)) S
+--   end.
+
+-- (** The soundness of the analysis follows. *)
+
+-- Ltac inv H := inversion H; clear H; subst.
+
+-- Lemma Cexec_sound:
+--   forall c s1 s2 S1,
+--   cexec s1 c s2 -> matches s1 S1 -> matches s2 (Cexec S1 c).
+-- Proof.
+--   induction c; intros s1 s2 S1 EXEC AG; cbn [Cexec].
+-- - (* SKIP *)
+--   inv EXEC. auto.
+-- - (* ASSIGN *)
+--   inv EXEC. apply matches_update. auto. apply Aeval_sound. auto.
+-- - (* SEQ *)
+--   inv EXEC. apply IHc2 with s'; auto. apply IHc1 with s1; auto.
+-- - (* IFTHENELSE *)
+--   inv EXEC.
+--   destruct (Beval S1 b) as [[]|] eqn:BE.
+--   + erewrite Beval_sound in H4 by eauto. apply IHc1 with s1; auto.
+--   + erewrite Beval_sound in H4 by eauto. apply IHc2 with s1; auto.
+--   + destruct (beval s1 b).
+--     * eapply matches_Le. apply Le_Join_l. eapply IHc1; eauto.
+--     * eapply matches_Le. apply Le_Join_r. eapply IHc2; eauto.
+-- - (* WHILE *)
+--   set (F := fun x => Join S1 (Cexec x c)).
+--   set (X := fixpoint F S1).
+--   assert (INNER: forall s1 c1 s2,
+--                  cexec s1 c1 s2 ->
+--                  c1 = WHILE b c ->
+--                  matches s1 X ->
+--                  matches s2 X).
+--   { induction 1; intros EQ AG1; inv EQ.
+--   - (* WHILE stop *)
+--     auto.
+--   - (* WHILE loop *)
+--     apply IHcexec2; auto.
+--     unfold X. eapply matches_Le. apply fixpoint_sound.
+--     unfold F. eapply matches_Le. apply Le_Join_r.
+--     apply IHc with s. auto. fold F. fold X. auto.
+--   }
+--   eapply INNER; eauto.
+--   unfold X. eapply matches_Le. apply fixpoint_sound.
+--   unfold F. eapply matches_Le. apply Le_Join_l.
+--   auto.
+-- Qed.
+
+
+
+-- (** ** 8.3 The constant propagation optimization *)
+
+-- (** We can use the results of the static analysis to simplify expressions
+--   further, replacing variables with known values by these values, then
+--   applying the smart constructors. *)
+
+-- Fixpoint cp_aexp (S: Store) (a: aexp) : aexp :=
+--   match a with
+--   | CONST n => CONST n
+--   | VAR x => match IdentMap.find x S with Some n => CONST n | None => VAR x end
+--   | PLUS a1 a2 => mk_PLUS (cp_aexp S a1) (cp_aexp S a2)
+--   | MINUS a1 a2 => mk_MINUS (cp_aexp S a1) (cp_aexp S a2)
+--   end.
+
+-- Fixpoint cp_bexp (S: Store) (b: bexp) : bexp :=
+--   match b with
+--   | TRUE => TRUE
+--   | FALSE => FALSE
+--   | EQUAL a1 a2 => mk_EQUAL (cp_aexp S a1) (cp_aexp S a2)
+--   | LESSEQUAL a1 a2 => mk_LESSEQUAL (cp_aexp S a1) (cp_aexp S a2)
+--   | NOT b => mk_NOT (cp_bexp S b)
+--   | AND b1 b2 => mk_AND (cp_bexp S b1) (cp_bexp S b2)
+--   end.
+
+-- (** Under the assumption that the concrete store matchess with the abstract store,
+--   these optimized expressions evaluate to the same values as the original
+--   expressions. *)
+
+-- Lemma cp_aexp_sound:
+--   forall s S, matches s S ->
+--   forall a, aeval s (cp_aexp S a) = aeval s a.
+-- Proof.
+--   intros s S AG; induction a; cbn.
+-- - auto.
+-- - destruct (IdentMap.find x S) as [n|] eqn:FIND.
+--   + symmetry. apply AG. auto.
+--   + auto.
+-- - rewrite mk_PLUS_sound, IHa1, IHa2. auto.
+-- - rewrite mk_MINUS_sound, IHa1, IHa2. auto.
+-- Qed.
+
+-- Lemma cp_bexp_sound:
+--   forall s S, matches s S ->
+--   forall b, beval s (cp_bexp S b) = beval s b.
+-- Proof.
+--   intros s S AG; induction b; cbn.
+-- - auto.
+-- - auto.
+-- - rewrite mk_EQUAL_sound, ! cp_aexp_sound by auto. auto.
+-- - rewrite mk_LESSEQUAL_sound, ! cp_aexp_sound by auto. auto.
+-- - rewrite mk_NOT_sound, IHb. auto.
+-- - rewrite mk_AND_sound, IHb1, IHb2. auto.
+-- Qed.
+
+-- (** The optimization of commands consists in propagating constants
+--   in expressions and simplifying the expressions, as above.
+--   In addition, conditionals and loops whose conditions are statically
+--   known will be simplified too, thanks to the smart constructors.
+
+--   The [S] parameter is the abstract store "before" the execution of [c].
+--   When recursing through [c], it must be updated like the static analysis
+--   [Cexec] does.  For example, if [c] is [SEQ c1 c2], [c2] is optimized
+--   using [Cexec S c1] as abstract store "before".  Likewise, if
+--   [c] is a loop [WHILE b c1], the loop body [c1] is optimized using
+--   [Cexec S (WHILE b c1)] as the abstract store "before".
+-- *)
+
+-- Fixpoint cp_com (S: Store) (c: com) : com :=
+--   match c with
+--   | SKIP => SKIP
+--   | ASSIGN x a =>
+--       ASSIGN x (cp_aexp S a)
+--   | SEQ c1 c2 =>
+--       SEQ (cp_com S c1) (cp_com (Cexec S c1) c2)
+--   | IFTHENELSE b c1 c2 =>
+--       mk_IFTHENELSE (cp_bexp S b) (cp_com S c1) (cp_com S c2)
+--   | WHILE b c =>
+--       let sfix := Cexec S (WHILE b c) in
+--       mk_WHILE (cp_bexp sfix b) (cp_com sfix c)
+--   end.
+
+-- (** Example: let's "optimize" Euclidean division under the dubious assumption
+--   that the divisor is 0... *)
+
+-- Compute (cp_com (Update "b" (Some 0) Top) Euclidean_division).
+
+-- (** Result is (in pseudocode):
+-- <<
+--      r := a;
+--      q := 0;
+--      while 0 <= r do
+--        r := r; q := q + 1
+--      done
+-- >>
+-- *)
+
+-- (** The proof of semantic preservation needs an unusual induction pattern:
+--   structural induction on the command [c], plus an inner induction
+--   on the number of iterations if [c] is a loop [WHILE b c1].
+--   This pattern follows closely the structure of the abstract interpreter
+--   [Cexec]: structural induction on the command + local fixpoint for loops. *)
+
+-- Lemma cp_com_correct_terminating:
+--   forall c s1 s2 S1,
+--   cexec s1 c s2 -> matches s1 S1 -> cexec s1 (cp_com S1 c) s2.
+-- Proof.
+--   induction c; intros s1 s2 S1 EXEC AG; cbn [cp_com].
+-- - (* SKIP *)
+--   auto.
+-- - (* ASSIGN *)
+--   inv EXEC. replace (aeval s1 a) with (aeval s1 (cp_aexp S1 a)).
+--   apply cexec_assign.
+--   apply cp_aexp_sound; auto.
+-- - (* SEQ *)
+--   inv EXEC. apply cexec_seq with s'.
+--   apply IHc1; auto.
+--   apply IHc2; auto. apply Cexec_sound with s1; auto.
+-- - (* IFTHENELSE *)
+--   inv EXEC.
+--   apply cexec_mk_IFTHENELSE.
+--   rewrite cp_bexp_sound by auto.
+--   destruct (beval s1 b); auto.
+-- - (* WHILE *)
+--   set (X := Cexec S1 (WHILE b c)).
+--   assert (INNER: forall s1 c1 s2,
+--                  cexec s1 c1 s2 ->
+--                  c1 = WHILE b c ->
+--                  matches s1 X ->
+--                  cexec s1 (mk_WHILE (cp_bexp X b) (cp_com X c)) s2).
+--   { induction 1; intros EQ AG1; inv EQ.
+--   - (* WHILE stop *)
+--     apply cexec_mk_WHILE_done. rewrite cp_bexp_sound by auto. auto.
+--   - (* WHILE loop *)
+--     apply cexec_mk_WHILE_loop with s'. rewrite cp_bexp_sound by auto. auto.
+--     apply IHc; auto.
+--     apply IHcexec2; auto.
+--     unfold X. cbn [Cexec].
+--     eapply matches_Le. apply fixpoint_sound.
+--     eapply matches_Le. apply Le_Join_r.
+--     apply Cexec_sound with s; auto.
+--   }
+--   eapply INNER; eauto.
+--   unfold X. cbn [Cexec].
+--   eapply matches_Le. apply fixpoint_sound.
+--   eapply matches_Le. apply Le_Join_l. auto.
+-- Qed.
